%!TEX root=../main.tex
\section{Derivation of the inertia of the clouds} % (fold)
\label{sec:derivation_of_the_inertia_of_the_clouds}

In this Section, we derive the inertia of the cloud $\CN$. Recall that 
\begin{equation}\label{eq:var_appendix}
    \Var\{\Xp{p}(t_p)\} = \sum_{n = 1}^N \pi_n \{\Xnp(t_p)\}^2 - \{\mup{p}(t_p)\}^2 \quad\text{where}\quad \mup{p}(t_p) = \sum_{n = 1}^N \pi_n\Xnp(t_p), \quad t_p \in \TT{p}.
\end{equation}

\begin{align*}
    \sum_{n = 1}^N \pi_n d^2(X_n, \mu) &= \sum_{n = 1}^N \pi_n \sum_{p = 1}^P\normLp{\Xnp - \mu^{(p)}}^2\\
    &= \sum_{p = 1}^P\left(\sum_{n = 1}^N \pi_n \normLp{\Xnp}^2 - \normLp{\mup{p}}^2\right) \\
    &= \sum_{p = 1}^P \int_{\TT{p}}\Var{\Xp{p}(t_p)} \dd t_p \\
\sum_{i = 1}^N \sum_{j = 1}^N \pi_i \pi_j d^2(X_i, X_j) &= \sum_{i = 1}^N \sum_{j = 1}^N \pi_i \pi_j \sum_{p = 1}^P \normLp{\Xp{p}_i - \Xp{p}_j}^2\\
    &= \sum_{p = 1}^P \left(2\sum_{i = 1}^N \pi_i\normLp{\Xp{p}_i}^2 - 2\sum_{i = 1}^N \sum_{j = 1}^N \inLp{\Xp{p}_i}{\Xp{p}_j}\right) \\
    &= \sum_{p = 1}^P \left(2\sum_{i = 1}^N \pi_i\normLp{\Xp{p}_i}^2 - 2\normLp{\mup{p}}^2 - 2\sum_{i = 1}^N \sum_{j = 1}^N \inLp{\Xp{p}_i}{\Xp{p}_j} + 2\normLp{\mup{p}}^2\right) \\
    &= 2\sum_{p = 1}^P \int_{\TT{p}}\Var{\Xp{p}(t_p)} \dd t_p
\end{align*}


% section derivation_of_the_inertia_of_the_clouds (end)